### Chain rule

###### Auther:Czhuman

Now we have a problem, when we encounter more complex functions how do we go about deriving them?

For example, y=ax+bx, how to find the derivative?

You can also do it the stupid way
$$
\begin{array}{ll}
y=ax+bx\\
y+\Delta y=a(x+\Delta x)+b(x+\Delta x)\\
y+\Delta y=ax+a\Delta x+bx+b\Delta x\\
\Delta y=a\Delta x+b\Delta x\\
\Delta y=(a+b)\Delta x\\
\frac{\Delta y}{\Delta x}=a+b\\
y'=a+b
\end{array}
$$
Too much trouble too much trouble!

So is there some kind of theorem that can help us deal with this situation better?

The answer is yes, and it is very practical.
$$
y=f(x)+g(x)\\
\frac{\Delta y}{\Delta x}=\frac{\Delta f}{\Delta x}+\frac{\Delta g}{\Delta x}
$$
This is the use of this rule for additive derivatives of functions.

Substituting into the above equation, it is easy to derive the derivative of y=ax+bx as a+b

Next, let's look at the derivative of the function multiplication:y=2x^2

As usual, we still try to use the stupid method
$$
\begin{array}{ll}
y=2x^2\\
y+\Delta y=2(x+\Delta x)^2\\
y+\Delta y=2x^2+4\,\Delta x\, x+2 \Delta x^2\\
\Delta y=4\,\Delta x\, x+2 \Delta x^2\\
\frac{\Delta y}{\Delta x}=4x+2\Delta x\\
\lim_{\Delta x \to 0}4x+2\Delta x=4x\\
y'=4x
\end{array}
$$
It's still a very complicated method.

Once again, another law is introduced:
$$
y=f(x)*g(x)\\
\frac{\Delta y}{\Delta x}=\frac{\Delta f}{\Delta x}g(x)+f(x)\frac{\Delta g}{\Delta x}
$$
Bring in the calculation again
$$
y=2x^2\\
y'=0*2x+2*2x=4x
$$
Obviously much simpler

Next we look at a nested function derivative
$$
y=\sin{x^2}
$$
In this case, we don't seem to be able to use our stupid solution.

But we can first wrap the inner function as Î”h
$$
y=f(g(x))\\
\frac{\Delta y}{\Delta x}=\frac{\Delta f}{\Delta h}\frac{\Delta h}{\Delta x}(h=g(x))
$$
Substitute again to calculate
$$
y=\sin{x^2}\\
y'=cos(x^2)2x
$$
As for the derivative of sin, I will explain it in detail in the next section.

We have mastered the three theorems of the chain rule, next, we can happily peel the onion skin of the derivative
